prove Cin_iff_CEin_CEin'

Computability/Constructions/Basic.lean
@@ -77,6 +77,7 @@ theorem Nat.RecursiveIn.ite {O:ℕ→ℕ} {f g:ℕ→.ℕ} {c:ℕ→ℕ} (hc:Nat
   simp [hcc, hca, hcb]
 
 
+-- like c_if_le_te, but allows either branch to diverge
 def c_if_le_te' (c1 c2 c3 c4:Code) := c_ite (c_sub.comp₂ c1 c2) c3 c4
 @[simp] theorem c_if_le_te'_ev (hc1:code_total O c1) (hc2:code_total O c2) : eval O (c_if_le_te' c1 c2 c3 c4) x = if (eval O c1 x).get (hc1 x) ≤ (eval O c2 x).get (hc2 x) then (eval O c3 x) else (eval O c4 x) := by
   simp [c_if_le_te']
@@ -89,6 +90,18 @@ def c_if_le_te' (c1 c2 c3 c4:Code) := c_ite (c_sub.comp₂ c1 c2) c3 c4
   simp [Part.Dom.bind $ hc1 x]
   simp [Part.Dom.bind $ hc2 x]
   exact Nat.sub_eq_zero_iff_le
+
+-- like c_if_eq_te, but allows either branch to diverge
+def c_if_eq_te' (c1 c2 c3 c4:Code) := c_ite (c_dist.comp₂ c1 c2) c3 c4
+@[simp] theorem c_if_eq_te'_ev (hc1:code_total O c1) (hc2:code_total O c2) : eval O (c_if_eq_te' c1 c2 c3 c4) x = if (eval O c1 x).get (hc1 x) = (eval O c2 x).get (hc2 x) then (eval O c3 x) else (eval O c4 x) := by
+  simp [c_if_eq_te']
+  have : code_total O (c_dist.comp₂ c1 c2) := by
+    apply total_comp_of $ prim_total c_dist_prim
+    apply total_pair_of hc1 hc2
+  simp [this]
+  simp [Seq.seq]
+  simp [Part.Dom.bind $ hc1 x]
+  simp [Part.Dom.bind $ hc2 x]
 
 
 def c_ifdom (c a:Computability.Code) := c_add.comp₂ (zero.comp c) a
