Computability/Post.lean
@@ -11,14 +11,14 @@ theorem partfun_eq_χgraph {f:ℕ→ℕ} : f ≡ᵀᶠ χ (total_graph f) := by 
 
 
 /-- `CEin O A` means that `A` is c.e. in `O`. -/
-def CEin (O:Set ℕ) (A:Set ℕ) : Prop := ∃ c:ℕ, A = W O c
+def CEin (O:Set ℕ) (A:Set ℕ) : Prop := ∃ c:Code, A = W O c
 @[simp] abbrev CE (A:Set ℕ) := CEin ∅ A
 @[simp] theorem CEin_trivial : CEin O (W O a) := exists_apply_eq_apply' (W O) a
 theorem CEIn_deg (h:CEin O A) : A ≤ᵀ O⌜ := by
   rcases h with ⟨c,h⟩
   rw [h]
   exact W_le_Jump c
-theorem CEin_range : CEin O A ↔ ∃ c:ℕ, A = WR O c := by
+theorem CEin_range : CEin O A ↔ ∃ c, A = WR O c := by
   simp only [CEin]
   constructor
   · intro h
@@ -62,17 +62,108 @@ theorem Cin_iff_Cin' : A≤ᵀB ↔ Aᶜ≤ᵀB := by
   simp at this
   exact this
 
-
-
-
+theorem asdoai (p:Part ℕ) (d:p.Dom) (h:p.get d=x) : p = Part.some x := by
+  exact Part.get_eq_iff_eq_some.mp h
 
 theorem Cin_iff_CEin_CEin' : A≤ᵀB ↔ (CEin B A ∧ CEin B Aᶜ) := by
   constructor
-  intro h
-  simp [CEin]
-  have := reducible_imp_W h
-  simp [reducible_iff_code] at h
-  sorry
+  -- first, the trivial direction.
+  · intro h
+    simp [CEin]
+    have h1 := reducible_imp_W h
+    have h2 := reducible_imp_W $ Cin_iff_Cin'.mp h
+    rcases h1 with ⟨c1, hc1⟩
+    rcases h2 with ⟨c2, hc2⟩
+    exact ⟨⟨c1, hc1.symm⟩,⟨c2, hc2.symm⟩⟩
+
+  intro ⟨h1,h2⟩
+  apply reducible_iff_code.mpr
+  rcases h1 with ⟨c1,hc1⟩
+  rcases h2 with ⟨c2,hc2⟩
+
+  let d := (
+    c_ite right
+    (zero.comp $ c2.comp left) $
+    c_if_eq_te' right (c_const 1)
+    (zero.comp $ c1.comp left)
+    c_diverge
+  )
+  /-
+  d is a program that does the following.
+  d(x,y):
+    if y=0:
+      run [c2](x)
+      return 0
+    elif y=1:
+      run [c1](x)
+      return 0
+    else:
+      diverge
+
+  Note that dovetailing d, will return 0 if x∉A and 1 if x∈A.
+  -/
+  use dovetail d
+  funext x
+
+  -- a1,a2: to be supplied as arguments for c_if_eq_te'_ev
+  have a1 : code_total (χ B) (right) := by exact fun x ↦ trivial
+  have a2 : code_total (χ B) (c_const 1) := by simp [code_total]
+
+  by_cases hx:x∈A
+  ·
+    have dvtthm := @dovetail_ev_0 (χ B) d x ?_
+    extract_lets at dvtthm; expose_names
+    all_goals
+      have tc1 : (eval (χ B) c1 x).Dom := by
+        simp [W, evalSet, PFun.Dom] at hc1
+        simp [hc1] at hx
+        exact hx
+      have tc2 : (eval (χ B) c2 x) = Part.none := by
+        have : ¬x∈Aᶜ := fun a ↦ a hx
+        simp [W, evalSet, PFun.Dom] at hc2
+        simp [hc2] at this
+        exact Part.eq_none_iff'.mpr this
+    rotate_left
+    · apply dovetail_ev_2.mpr
+      simp [d, c_if_eq_te'_ev a1 a2, eval, Part.Dom.bind $ tc1]
+      exact ⟨1,rfl⟩
+    ·
+      simp [χ, hx]
+      simp [d, c_if_eq_te'_ev a1 a2, eval, Part.Dom.bind $ tc1, tc2] at dvtthm
+
+      have : dvt = 1 := by
+        contrapose dvtthm
+        simp [dvtthm]
+      simp [dvt] at this
+      exact Part.get_eq_iff_eq_some.mp this
+  ·
+    have hx' : x∈Aᶜ := hx
+    have dvtthm := @dovetail_ev_0 (χ B) d x ?_
+    extract_lets at dvtthm; expose_names
+    all_goals
+      have tc1 : (eval (χ B) c2 x).Dom := by
+        simp [W, evalSet, PFun.Dom] at hc2
+        simp [hc2] at hx'
+        exact hx'
+      have tc2 : (eval (χ B) c1 x) = Part.none := by
+        simp [W, evalSet, PFun.Dom] at hc1
+        simp [hc1] at hx
+        exact Part.eq_none_iff'.mpr hx
+    rotate_left
+    · apply dovetail_ev_2.mpr
+      simp [d, c_if_eq_te'_ev a1 a2, eval, Part.Dom.bind $ tc1]
+      exact ⟨0,fun a ↦ False.elim (a rfl)⟩
+    ·
+      simp [χ, hx]
+      simp [d, c_if_eq_te'_ev a1 a2, eval, Part.Dom.bind $ tc1, tc2] at dvtthm
+
+      have : dvt = 0 := by
+        contrapose dvtthm
+        simp [dvtthm]
+      simp [dvt] at this
+      exact Part.get_eq_iff_eq_some.mp this
+
+
 
 
 /-- immuneIn O A := A is immune in O -/
